datatypes.v
@@ -221,12 +221,12 @@ Inductive asfs_map_val : Type :=
   | ASFSBasicVal (val: asfs_stack_val)
   | ASFSOp (opcode : oper_label) (args : list asfs_stack_val).
   
-Inductive flat_asfs_map_val : Type :=
-  | FASFSBasicVal (val: asfs_stack_val)
-  | FASFSOp (opcode : oper_label) (args : list flat_asfs_map_val).
+  
+Inductive stack_expr : Type :=
+  | UVal (val: EVMWord)
+  | UInStackVar (var: nat)
+  | UOp (opcode : oper_label) (args : list stack_expr).
 
-Definition concrete_stack := list EVMWord.
-Definition in_stack := list nat.
 Definition asfs_stack  := list asfs_stack_val.
 Definition asfs_map    := list (nat*asfs_map_val).
 
